---
title: "MAT232: Calculus of Several Variables"
image: curve.png
categories: [Multivariable Calculus, Linear Algebra, Vector Calculus]
description: 'Notes for MAT232 Summer 2025'
toc-depth: 1
---

This page contains tutorial notes for [MAT232H5 Calculus of Several Variables](https://utm.calendar.utoronto.ca/course/mat232h5%5D) Summer 2025 under the instruction of [Dr. Elio Mazzeo](https://www.utm.utoronto.ca/math-cs-stats/people/elio-mazzeo).

# Week 1

Week 1 tutorial notes [Here](/teaching/MAT232H5-Summer-2025/week1.pdf){download="week1"}

# Week 2

Week 2 tutorial notes [Here](/teaching/MAT232H5-Summer-2025/week2.pdf){download="week2"}

## Parametric Equations

Suppose there is a third variable $t$ (called a parameter), we can *parameterize* $x$ and $y$ by the equations \begin{align*}
x &= f(t) \\
y &= y(t)
\end{align*} where $a \le t \le b$ which has initial point $(f(a), g(a))$ and terminal point $(f(b), g(b))$.

Now, we would like to find derivatives and compute arclengths of the parametric curves, much like we did with functions. Suppose that $f,g$ are differentiable functions and we need to find the tangent line at a point on the parametric curve $x = f(t)$ and $y = g(t)$, where y is also a differentiable function of $x$. If $dx/dt \ne 0$, then the slopes of the parametric curve is given by \begin{align*}
\frac{dy}{dx} = \frac{dy/dt}{dx/dt}
\end{align*}

Furthermore suppose that $y$ is a twice differentiable function of $x$, then at any point $dx/dt \ne 0$ and \begin{align*}
\frac{d^2y}{dx^2} 
&= \frac{d}{dx} \left( \frac{dy}{dx} \right) = \frac{ \dfrac{d}{dt} \left( \dfrac{dy}{dx} \right) }{ \dfrac{dx}{dt} }
\end{align*}

Suppose that a curve C can be described by the parametric equations $x = f(t)$ and $y = g(t)$, where $\alpha \le t \le \beta$. Additionally, suppose that $f', g'$ are continuous in $\alpha \le t \le \beta$. Then the length of C is given by \begin{align*}
L = \int_{\alpha}^{\beta} \sqrt{ \left( \frac{dx}{dt} \right)^2 + \left( \frac{dy}{dt} \right)^2 } \, dt
\end{align*}

# Week 3

Week 3 tutorial notes [Here](/teaching/MAT232H5-Summer-2025/week3.pdf){download="week3"}

## Polar Coordinates

So far we have been working exclusively in the Cartesian/rectangular coordinate system. As we will see in the near future, this is not always the easiest coordinate system to work in. In this section, we will introduce the polar coordinate system.

\begin{align*}
x &= r \cos{\theta}, \hspace{0.5cm} y = r \sin{\theta} \\
r^2 &= x^2 + y^2, \hspace{0.5cm} \tan{\theta} = \frac{y}{x}
\end{align*}

The second line of equation is used to help convert back and forth from the Cartesian coordinate system and the polar coordinate system.

To find a tangent line to the polar curve $r = f{(\theta)}$, we regard $\theta$ as a parameter and write its parametric equations as

\begin{align*}
x = r \cos{\theta} = f(\theta) \cos{\theta}, \hspace{0.5cm} y = r \sin{\theta}\sin{(\theta)} \\
\end{align*}

Then following the equation of slope for parametric curves and the product rule,

$$\frac{dy}{dx} = \frac{dy/d \theta}{dx/ d \theta} = \frac{\frac{dr}{d \theta} \sin{\theta} + r \cos{\theta}}{\frac{dr}{d \theta} \cos{\theta} - r \sin{\theta}}$$

We can locate horizontal tangents by finding points where $dy/d\theta = 0$ given that $dx/d\theta \ne 0$. Likewise, vertical tangents can be found where $dx/d\theta = 0$ given that $dy/d\theta \ne 0$.

## Equation of a Parabola, Ellipse, Hyperbola, and Sphere

Parabola: \begin{align*}
x^2 = 4py, \hspace{0.5cm} \text{or} \hspace{0.5cm} y^2 = 4px  \\
\end{align*}

Ellipse: \begin{align*}
\frac{x^2}{a^2} + \frac{y^2}{b^2} &= 1, \hspace{0.5cm} \text{where} \hspace{0.5cm} a \ge b > 0  \hspace{0.5cm} \text{or} \\
\frac{x^2}{b^2} + \frac{y^2}{a^2} &= 1, \hspace{0.5cm} \text{where} \hspace{0.5cm} a \ge b > 0 
\end{align*}

Hyperbola: \begin{align*}
\frac{x^2}{a^2} - \frac{y^2}{b^2} &= 1, \hspace{0.5cm} \text{where} \hspace{0.5cm} a \ge b > 0  \hspace{0.5cm} \text{or} \\
\frac{y^2}{b^2} - \frac{x^2}{a^2} &= 1, \hspace{0.5cm} \text{where} \hspace{0.5cm} a \ge b > 0 
\end{align*}

Sphere: \begin{align*}
(x-h)^2 + (y-k)^2 + (z-l)^2 = r^2 \hspace{0.5cm} \text{where the center is located at $(h, k, l)$ with radius $r$}
\end{align*}

## Linear Algebra in 3D (Part I)

In 3D space, a point is represented as $(x, y, z)$.

An equation in terms of $x$ and $y$ defines a curve in the 2D space $\mathbb{R}^2$, while an equation in terms of $x, y$ and $z$ defines a surface in 3D space $\mathbb{R}^3$.

Given two points $P(x_1, y_1, z_1)$ and $Q(x_2, y_2, z_2)$, the distance between them is: \begin{align*}
|PQ| = \sqrt{(x_2 - x_1)^2 + (y_2 - y_1)^2 + (z_2 - z_1)^2} \\
\end{align*}

A vector is a quantity with both magnitude and direction. Given two points $P$ and $Q$, the vector from $P$ to $Q$ is defined by the difference of their coordinates: \begin{align*}
\bar{a} = \langle x_2 - x_1,\, y_2 - y_1,\, z_2 - z_1 \rangle
\end{align*}

To find the magnitude (or norm) of a vector $\vec{a} = (a_1, a_2, a_3) \in \mathbb{R}^3$, we compute: $$|\vec{a}| = \sqrt{a_1^2 + a_2^2 + a_3^2}$$ The standard basis vectors in $\mathbb{R}^3$ is given by $$
\vec{i} = \langle 1, 0, 0 \rangle, \quad
\vec{j} = \langle 0, 1, 0 \rangle, \quad
\vec{k} = \langle 0, 0, 1 \rangle
$$

This is particularly useful as any vector in $\mathbb{R}^3$ can be written as: $$\vec{a} = a_1\vec{i} + a_2\vec{j} + a_3\vec{k}$$

A unit vector is any vector with magnitute of $1$. The standard basis is an example of a unit vector. To convert any vector into a unit vector: $$\vec{u} = \frac{\vec{a}}{|\vec{a}|} = \frac{\vec{a}}{\|\vec{a}\|} = \frac{\vec{a}}{\sqrt{a_1^2 + a_2^2 + a_3^2}}$$

# Week 4

Week 4 tutorial notes [Here](/teaching/MAT232H5-Summer-2025/week4.pdf){download="week4"}

## Linear Algebra in 3D (Part II)

In this section, we continue from last week's discussion about linear algebra in $\mathbb{R}^3$ by introducing the dot product, cross product, and the forms of equations of lines and planes.

Let $\vec{a} = \langle a_1, a_2, a_3 \rangle$ and $\vec{b} = \langle b_1, b_2, b_3 \rangle$. The dot product is given by $$\vec{a} \cdot \vec{b} = \langle a_1, a_2, a_3 \rangle \cdot \langle b_1, b_2, b_3 \rangle
= a_1 b_1 + a_2 b_2 + a_3 b_3$$

Alternatively, if $\theta$ is an angle between non-zero vectors $\vec{a}$ and $\vec{b}$, then $$\vec{a} \cdot \vec{b} = |\vec{a}| |\vec{b}| \cos(\theta)$$

::: callout-note
**Theorem: Orthogonality and Dot Product**.

Two non-zero vectors are $\vec{a}$ and $\vec{b}$ are orthogonal if and only if $\vec{a} \cdot \vec{b} = 0$
:::

Let $\vec{a} = \langle a_1, a_2, a_3 \rangle$ and $\vec{b} = \langle b_1, b_2, b_3 \rangle$. Then the cross product is given by $$\vec{c} = \vec{a} \times \vec{b} = \langle a_2 b_3 - a_3 b_2,\ a_3 b_1 - a_1 b_3,\ a_1 b_2 - a_2 b_1 \rangle$$ Note that this formula comes from the determinant of a matrix

$$\vec{c} = \vec{a} \times \vec{b} = 
\left|
\begin{array}{ccc}
\vec{i} & \vec{j} & \vec{k} \\
a_1 & a_2 & a_3 \\
b_1 & b_2 & b_3 \\
\end{array}
\right|
= \vec{i}
\left|
\begin{array}{cc}
a_2 & a_3 \\
b_2 & b_3 \\
\end{array}
\right|
- \vec{j}
\left|
\begin{array}{cc}
a_1 & a_3 \\
b_1 & b_3 \\
\end{array}
\right|
+ \vec{k}
\left|
\begin{array}{cc}
a_1 & a_2 \\
b_1 & b_2 \\
\end{array}
\right|$$

::: callout-note
**Theorem: Orthogonality and Cross Product**.

The vector $\vec{c}$ is orthogonal to both vectors $\vec{a}$ and $\vec{b}$.
:::

::: callout-note
**Theorem: Geometric Interpretation of the Cross Product**.

If $0 \le \theta \le \pi$ is an angle between $\vec{a}$ and $\vec{b}$, then $$|\vec{a} \times \vec{b}| = |\vec{a}|\, |\vec{b}| \sin(\theta)$$

Furthermore, $\vec{a}$ and $\vec{b}$ are parallel if and only if $\vec{a} \times \vec{b} = \vec{0}$.
:::

We now look at the equation of a line in $\mathbb{R}^3$. Note that the equation $y = mx+b$ does not describe a line anymore in $\mathbb{R}^3$, but rather a plane. For now, we introduce two ways to describe a line in $\mathbb{R}^3$

The vector form of the equation of a line is given by

$$r = \vec{r}_0 + t \vec{v} = \langle x_0, y_0, z_0 \rangle + t \langle a, b, c \rangle$$ where

-   $\vec{r}$: a general position vector to any point on the line.\
-   $\vec{r}_0 = \langle x_0, y_0, z_0 \rangle$: a fixed point (starting point) on the line.\
-   $\vec{v} = \langle a, b, c \rangle$: a direction vector that gives the direction of the line.\
-   $t \in \mathbb{R}$: a scalar parameter.

Alternatively, the line can also be represented using its parametric equations, given by:

\begin{aligned}
x &= x_0 + ta \\
y &= y_0 + tb \\
z &= z_0 + tc
\end{aligned}

where

-   $(x_0, y_0, z_0)$: a known point on the line (starting point).\
-   $(a, b, c)$: direction vector components — the direction in which the line extends.\
-   $t \in \mathbb{R}$: a scalar parameter.

Note that the parametric equations can be derived by equating each component from the vector form of the line.

Lastly, we look at the equation of a plane in $\mathbb{R}^3$. We also introduce two ways to describe a plane.

The vector equation of the plane is

$$\vec{n} \cdot \langle \vec{r} - \vec{r}_0 \rangle = \vec{0}$$

where

-   $\vec{n} = \langle a, b, c \rangle$: a normal vector perpendicular to the plane.\
-   $\vec{r} = \langle x, y, z \rangle$: a general position vector to a point on the plane.\
-   $\vec{r}_0 = \langle x_0, y_0, z_0 \rangle$: a known point on the plane.

The scalar equation of the plane is $$a(x - x_0) + b(y - y_0) + c(z - z_0) = 0$$

::: callout-note
**Example: Vector and Scalar Equations**.

Given: $$\vec{r}_0 = \langle 1, 2, 3 \rangle, \quad \vec{n} = \langle 4, -2, 5 \rangle, \quad \vec{r} = \langle x, y, z \rangle$$

The vector equation of the plane is: $$\vec{n} \cdot (\vec{r} - \vec{r}_0) = 0$$

Substitute the vectors: $$\langle 4, -2, 5 \rangle \cdot \left( \langle x, y, z \rangle - \langle 1, 2, 3 \rangle \right) = 0$$

Simplify: $$\langle 4, -2, 5 \rangle \cdot \langle x - 1, y - 2, z - 3 \rangle = 0$$

Dot product gives the scalar equation: $$4(x - 1) - 2(y - 2) + 5(z - 3) = 0 \quad \Rightarrow \quad 4x - 2y + 5z = 21$$
:::

# Week 5

Week 5 tutorial notes [Here](/teaching/MAT232H5-Summer-2025/week5.pdf){download="week5"}

## Vector Functions

A vector function is a function that takes one (or more) variables and returns a vector of functions. We will only discuss the case where the function takes one variable.

In $\mathbb{R}^3$, a single variable vector function have the form

$$\bar{r}(t) = \langle f(t), g(t), h(t) \rangle = f(t)\bar{i} + g(t)\bar{j} + h(t)\bar{k}$$ Let's now talk about limits, derivatives and integrals with vector functions. For the limit of a vector function,

$$\lim_{t \to a} \bar{r}(t) = \left\langle \lim_{t \to a} f(t), \lim_{t \to a} g(t), \lim_{t \to a} h(t) \right\rangle
\quad  \newline \text{assuming the limits of all the component functions exist.}$$

Furthermore, we say a vector function $\bar{r}(t)$ is continuous at $a$ if $\lim{t \to a} = \bar{r}(a)$.

Next, let's talk about the derivatives of vector functions. $$\frac{d\bar{r}}{dt} = \bar{r}'(t) = \lim_{h \to 0} \frac{\bar{r}(t+h) - \bar{r}(t)}{h}$$

Note that the derivative of a vector function is just the vector of the derivatives of its components. That is, $$\bar{r}'(t) = \langle f'(t), g'(t), h'(t) \rangle = f'(t)\bar{i} + g'(t)\bar{j} + h'(t)\bar{k}$$

::: callout-note
**Theorem: Differential Rules of Vector Functions**.

Suppose that $\vec{u}(t)$ and $\vec{v}(t)$ are differentiable vector functions, $c$ is a scalar, and $f$ is a real-valued function. Then, \begin{align}
&1.\quad \frac{d}{dt}[\vec{u}(t) + \vec{v}(t)] = \vec{u}'(t) + \vec{v}'(t) \\
&2.\quad \frac{d}{dt}[c \vec{u}(t)] = c \vec{u}'(t) \\
&3.\quad \frac{d}{dt}[f(t)\vec{u}(t)] = f'(t)\vec{u}(t) + f(t)\vec{u}'(t) \\
&4.\quad \frac{d}{dt}[\vec{u}(t) \cdot \vec{v}(t)] = \vec{u}'(t) \cdot \vec{v}(t) + \vec{u}(t) \cdot \vec{v}'(t) \\
&5.\quad \frac{d}{dt}[\vec{u}(t) \times \vec{v}(t)] = \vec{u}'(t) \times \vec{v}(t) + \vec{u}(t) \times \vec{v}'(t) \\
&6.\quad \frac{d}{dt}[\vec{u}(f(t))] = f'(t)\vec{u}'(f(t)) \\
\end{align}
:::

Given how neatly the limit and derivative rules extend to vector-valued functions, it's no surprise that similar rules apply to definite (and indefinite) integrals as well. \begin{align}
\int_a^b \vec{r}(t) , dt 
&= \left( \int_a^b f(t) , dt \right)\vec{i} + \left( \int_a^b g(t) , dt \right)\vec{j} + \left( \int_a^b h(t) , dt \right)\vec{k} \\
&= \left( F(t) \big|_a^b \right)\vec{i} + \left( G(t) \big|_a^b \right)\vec{j} + \left( H(t) \big|_a^b \right)\vec{k} \\
&= \left( F(b) - F(a) \right)\vec{i} + \left( G(b) - G(a) \right)\vec{j} + \left( H(b) - H(a) \right)\vec{k}
\end{align}

Finally, the arc length formula extends naturally to vector-valued functions and is given by: \begin{align}
L &= \int_a^b \sqrt{[f'(t)]^2 + [g'(t)]^2 + [h'(t)]^2} \, dt \\
  &= \int_a^b \sqrt{\left( \frac{dx}{dt} \right)^2 + \left( \frac{dy}{dt} \right)^2 + \left( \frac{dz}{dt} \right)^2} \, dt \\
  &= \int_a^b \left| \vec{r}\,'(t) \right| \, dt
\end{align}

# Week 6

Week 6 tutorial notes [TBP](){download="week5"}

## Functions of Two Variables

A function $f$ of two variables is a rule that assigns to each ordered pair of real numbers $(x, y)$ in a set $D$ a unique real number denoted by $f(x, y)$. The set $D$ is the domain of $f$ and its range is the set of values that $f$ takes on, that is, $$\{f(x,y) | (x,y) \in D\}$$ The graph of $f$ is the set of all points $(x, y, z) \in R^3$ such that $z = f(x, y)$ and $(x, y) \in D$.

To visualize $z = f(x,y)$, one method is to set the equation $f(x, y) = k$ where $k$ is a constant. Geometrically, they are like elevation lines on a topographic map where each level marks a specific height.

## Calculus with Functions of Two Variables

For a function $f(x, y)$, we define its first partial derivatives $f_x$ and $f_y$ as $$
f_x(x, y) = \lim_{h \to 0} \frac{f(x + h, y) - f(x, y)}{h}
\qquad
f_y(x, y) = \lim_{h \to 0} \frac{f(x, y + h) - f(x, y)}{h}
$$ provided that the limit(s) exists. Note its similarity to the definitions of the single variable case.

There are many alternate notations for partial derivatives. Below are some most common ones used

$$
\begin{aligned}
f_x(x, y) = f_x &= \frac{\partial f}{\partial x} = \frac{\partial}{\partial x} \left( f(x, y) \right) = z_x = \frac{\partial z}{\partial x} = D_x f \\
f_y(x, y) = f_y &= \frac{\partial f}{\partial y} = \frac{\partial}{\partial y} \left( f(x, y) \right) = z_y = \frac{\partial z}{\partial y} = D_y f
\end{aligned}
$$

To compute the derivative with respect to one variable $x$, we regard the other variable $y$ as constant and differentiate $f(x,y)$ with respect to $x$; the same applies when differentiating with respect to $y$.

When computing derivatives of second order, we use the following notation which can be extended to three or more variables. These are sometimes called mixed partial derivatives since we are taking derivatives with respect to more than one variable. $$
\begin{aligned}
(f_x)_x = f_{xx} = f_{11} &= \frac{\partial}{\partial x} \left( \frac{\partial f}{\partial x} \right) 
= \frac{\partial^2 f}{\partial x^2} = \frac{\partial^2 z}{\partial x^2} \\
(f_y)_x = f_{yx} = f_{21} &= \frac{\partial}{\partial x} \left( \frac{\partial f}{\partial y} \right) 
= \frac{\partial^2 f}{\partial x \partial y} = \frac{\partial^2 z}{\partial x \partial y} \\
(f_x)_y = f_{xy} = f_{12} &= \frac{\partial}{\partial y} \left( \frac{\partial f}{\partial x} \right) 
= \frac{\partial^2 f}{\partial y \partial x} = \frac{\partial^2 z}{\partial y \partial x} \\
(f_y)_y = f_{yy} = f_{22} &= \frac{\partial}{\partial y} \left( \frac{\partial f}{\partial y} \right) 
= \frac{\partial^2 f}{\partial y^2} = \frac{\partial^2 z}{\partial y^2}
\end{aligned}
$$

Note that the notation might be confusing at first glance, since sometimes it is read from left to right and others right to left.

In general, it is *not* true that $f_{xy} = f_{yx}$. However the below theorem states when this is satisfied.

::: callout-note
**Theorem: Clairaut’s Theorem**.

Suppose that $f$ is defined on a disk $D$ that contains the point $(a, b)$. If the functions $f_{x,y}$ and $f_{y, x}$ are both continuous on $D$, then $$f_{xy}(a,b) = f_{yx}(a,b)$$
:::

Lastly, if we suppose that $f$ has continuous partial derivatives, then an equation of the tangent plane to the surface $z = f(x, y)$ at the point $P(x_0, y_0, z_0)$ is $$z - z_0 = f_x(x_0, y_0)(x - x_0) + f_y(x_0, y_0)(y - y_0)$$
